LeanMathLogicExploration/RelationalAlgebraQuotient.lean
@@ -1,0 +1,90 @@
+-- Started working on this but it was too complicated and I don't know if I really need it.
+
+-- Define the quotient type for relations
+def RelationQuotient (α β : Type u) := Quotient (@instSetoidRelation α β)
+
+-- Lifts both arguments to the quotient.
+def RelationQuotient.le (R S : RelationQuotient α β) : Prop :=
+  Quotient.lift₂
+    (fun R S : Relation α β => R ≤ S)
+    (fun (R1 S1 R2 S2 : Relation α β) (eqR : ext_eq R1 R2) (eqS : ext_eq S1 S2) =>
+      let forward :  (R1 ≤ S1) → (R2 ≤ S2) := by
+        intro R1_le_S1
+        have R1_eq_R2 : eval R1 = eval R2 :=  Relation.eval_eq_iff_eq.mpr eqR
+        have S1_eq_S2 : eval S1 = eval S2 :=  Relation.eval_eq_iff_eq.mpr eqS
+        have conseqent := le_rel_iff_le_eval.mp R1_le_S1
+        rw [R1_eq_R2, S1_eq_S2] at conseqent
+        exact conseqent
+
+      let backward : (R2 ≤ S2) → (R1 ≤ S1) := by
+        intro R2_le_S2
+        have R2_eq_R1 : eval R2 = eval R1 :=  (Relation.eval_eq_iff_eq.mpr eqR).symm
+        have S2_eq_S1 : eval S2 = eval S1 :=  (Relation.eval_eq_iff_eq.mpr eqS).symm
+        have consequent := le_rel_iff_le_eval.mp R2_le_S2
+        rw [R2_eq_R1, S2_eq_S1] at consequent
+        exact consequent
+
+      let biImpl :  (R1 ≤ S1) ↔  (R2 ≤ S2) :=
+        ⟨forward, backward⟩
+
+      propext  biImpl
+    )
+    R S
+
+-- This sends relations to the quotient type based on the ext_eq equivalence
+def Relation.toQuotient (R : Relation α β) : RelationQuotient α β :=
+  Quotient.mk (α := Relation α β) (@instSetoidRelation α β) R
+
+ instance : LE (RelationQuotient α β) where
+    le R S := RelationQuotient.le R S
+
+-- def lift_rel_le {R S: Relation α β }(h: R ≤ S) : (toQuotient R) ≤ (toQuotient S)  := sorry
+
+
+theorem lift_rel_le {α β : Type u} {R S: Relation α β} (h: R ≤ S) : ( ⟦R⟧ ≤ ⟦S⟧) := by
+  unfold toQuotient
+
+
+  -- unfold  instLERelationQuotient.1 ⟦R⟧ ⟦S⟧
+
+  -- RelationQuotient.le
+
+  exact h
+
+-- Create PartialOrder instance
+-- A partial order is a pre-order plus anti-symmetry
+-- Now define the PartialOrder on the Quotient type
+instance : PartialOrder (RelationQuotient α β) where
+  le := RelationQuotient.le
+  lt := fun R S => RelationQuotient.le R S ∧ ¬RelationQuotient.le S R
+  le_refl := by
+    intro R
+    apply Quotient.ind R
+    intro R'
+    exact le_refl R'
+  le_trans := by
+    intro R S T
+    apply Quotient.ind R
+    intro R'
+    apply Quotient.ind S
+    intro S'
+    apply Quotient.ind T
+    intro T'
+    intro hRS hST
+    exact le_trans hRS hST
+  le_antisymm := by
+    intro R S
+    apply Quotient.ind R
+    intro R'
+    apply Quotient.ind S
+    intro S'
+    intro hRS hSR
+    apply Quotient.sound
+    exact ⟨hRS, hSR⟩
+  lt_iff_le_not_le := by
+    intro R S
+    apply Quotient.ind R
+    intro R'
+    apply Quotient.ind S
+    intro S'
+    exact ⟨fun h => ⟨h.1, h.2⟩, fun h => ⟨h.1, h.2⟩⟩
