LeanMathLogicExploration/RelationalPrograms.lean
@@ -1,0 +1,4 @@
+-- In this file I'm writing compositional formulas for common manipulations of relations.
+
+
+-- A selection relation is a subre
